cp

secure_api/aead/Crypto.AEAD.MAC_Wrapper.Invariant.fst
@@ -189,6 +189,92 @@ private let frame_plain_and_cipher
 	       Plain.sel_plain h0 plainlen plain == Plain.sel_plain h1 plainlen plain /\
 	       Buffer.as_seq h0 (cbuf ct) == Buffer.as_seq h1 (cbuf ct)))) = ()
 
+module CMAWrapper = Crypto.AEAD.Wrappers.CMA
+
+val mac_modifies_preserves_norm_keys
+  (#i:id)
+  (#j:CMA.id)
+  (#aadlen:aadlen_32)
+  (#plainlen:nz_ok_len_32 i)
+  (st:aead_state i Writer)
+  (n:Cipher.iv (alg i))
+  (aad:lbuffer (v aadlen))
+  (plain:plainBuffer i (v plainlen))
+  (ct:ctagbuf plainlen)
+  (ak:CMA.state (i, n))
+  (acc:CMA.accBuffer (i, n))
+  (h0 h1:mem)
+  (r:MAC.elemB j) : Lemma 
+  (requires ( let tag = Buffer.sub ct plainlen MAC.taglen in	
+              let b = MAC.as_buffer r in
+              enc_dec_separation st aad plain ct  /\
+              enc_dec_liveness st aad plain ct h0 /\
+              HS.(is_stack_region h0.tip) /\
+              Buffer.frameOf (MAC.as_buffer (CMA.abuf acc)) = HS.(h0.tip) /\
+              CMA.(ak.region = PRF.(st.prf.mac_rgn)) /\
+              CMAWrapper.mac_modifies i n tag ak acc h0 h1 /\
+              Buffer.frameOf b = PRF.(st.prf.mac_rgn) /\
+              fst j == i /\
+              MAC.norm_r h0 r))
+  (ensures (MAC.norm_r h1 r))
+#reset-options "--z3rlimit 100 --max_fuel 0 --max_ifuel 0"
+let mac_modifies_preserves_norm_keys #i #j #aadlen #plainlen st n aad plain ct ak acc h0 h1 r =
+  let open CMA in
+  let tag = Buffer.sub ct plainlen MAC.taglen in	
+  let abuf = MAC.as_buffer (abuf acc) in
+  let b = MAC.reveal_elemB r in
+  assert (Buffer.disjoint b tag);
+  assert (Buffer.disjoint b abuf);
+  match macAlg_of_id i with
+  | POLY1305 -> 
+    assert (Buffer.live h1 b);
+    assert (MAC.norm_r h1 r)
+  | GHASH -> 
+    assert (MAC.norm_r h1 r)
+
+val mac_preserves_prf_inv
+  (#i:id)
+  (#aadlen:aadlen_32)
+  (#plainlen:nz_ok_len_32 i)
+  (st:aead_state i Writer)
+  (n:Cipher.iv (alg i))
+  (aad:lbuffer (v aadlen))
+  (plain:plainBuffer i (v plainlen))
+  (ct:ctagbuf plainlen)
+  (ak:CMA.state (i, n))
+  (acc:CMA.accBuffer (i, n))
+  (h0 h1:mem) : Lemma 
+  (requires ( let tag = Buffer.sub ct plainlen MAC.taglen in	
+              enc_dec_separation st aad plain ct  /\
+              enc_dec_liveness st aad plain ct h0 /\
+              aead_liveness st h0 /\
+              HS.(is_stack_region h0.tip) /\
+              Buffer.frameOf (MAC.as_buffer (CMA.abuf acc)) = HS.(h0.tip) /\
+              CMA.(ak.region = PRF.(st.prf.mac_rgn)) /\
+              CMAWrapper.mac_modifies i n tag ak acc h0 h1 /\
+              (prf i ==> (
+                let blocks : prf_table st.prf.mac_rgn i = HS.sel h0 (itable i st.prf) in
+                prf_mac_inv blocks h0))))
+  (ensures (prf i ==>  (
+                let blocks : prf_table st.prf.mac_rgn i = HS.sel h1 (itable i st.prf) in
+                prf_mac_inv #i #st.prf.mac_rgn blocks h1)))
+let mac_preserves_prf_inv #i #aadlen #plainlen st n aad plain ct ak acc h0 h1 =
+  let open CMA in
+  if prf i then begin
+    let table = itable i st.prf in
+    let blocks_0 : prf_table st.prf.mac_rgn i = HS.sel h0 table in
+    let blocks_1 : prf_table st.prf.mac_rgn i = HS.sel h1 table in
+    assume (blocks_0 == blocks_1);
+    let h1 : (h:mem{prf i}) = h1 in
+    let aux (x:domain_mac i) : Lemma (PRF.prf_mac_inv blocks_1 x h1) =
+        match PRF.find_mac blocks_1 x with 
+        | None -> ()
+        | Some mc -> mac_modifies_preserves_norm_keys st n aad plain ct ak acc h0 h1 mc.r
+    in
+    FStar.Classical.forall_intro aux
+  end
+
+
 (*
  * propagating the invariant across mac_wrapper
  *)
